Realise I want other list range syntaxes, so add m ..< n variant.

hol/listRangeScript.sml
@@ -4,8 +4,8 @@ open listTheory
 
 val _ = new_theory "listRange";
 
-val listRange_def = Define`
-  listRange m n = GENLIST (\i. m + i) (n + 1 - m)
+val listRangeINC_def = Define`
+  listRangeINC m n = GENLIST (\i. m + i) (n + 1 - m)
 `;
 
 val _ = add_rule { block_style = (AroundEachPhrase, (PP.CONSISTENT, 0)),
@@ -14,33 +14,58 @@ val _ = add_rule { block_style = (AroundEachPhrase, (PP.CONSISTENT, 0)),
                    pp_elements = [TOK "[", TM, HardSpace 1, TOK "..",
                                   BreakSpace(1,1), TM, BreakSpace(0,0),
                                   TOK "]"],
-                   term_name = "listRange" }
+                   term_name = "listRangeINC" }
 
-val listRange_SING = store_thm(
-  "listRange_SING",
+val listRangeINC_SING = store_thm(
+  "listRangeINC_SING",
   ``[m .. m] = [m]``,
-  SIMP_TAC (srw_ss()) [listRange_def]);
-val _ = export_rewrites ["listRange_SING"]
+  SIMP_TAC (srw_ss()) [listRangeINC_def]);
+val _ = export_rewrites ["listRangeINC_SING"]
 
-val MEM_listRange = store_thm(
-  "MEM_listRange",
+val MEM_listRangeINC = store_thm(
+  "MEM_listRangeINC",
   ``MEM x [m .. n] <=> m <= x /\ x <= n``,
   SIMP_TAC (srw_ss() ++ ARITH_ss)
-           [listRange_def, MEM_GENLIST, EQ_IMP_THM] THEN
+           [listRangeINC_def, MEM_GENLIST, EQ_IMP_THM] THEN
   STRIP_TAC THEN Q.EXISTS_TAC `x - m` THEN DECIDE_TAC);
-val _ = export_rewrites ["MEM_listRange"]
+val _ = export_rewrites ["MEM_listRangeINC"]
 
-val listRange_CONS = store_thm(
-  "listRange_CONS",
+val listRangeINC_CONS = store_thm(
+  "listRangeINC_CONS",
   ``m <= n ==> ([m .. n] = m :: [m+1 .. n])``,
-  SIMP_TAC (srw_ss()) [listRange_def] THEN STRIP_TAC THEN
+  SIMP_TAC (srw_ss()) [listRangeINC_def] THEN STRIP_TAC THEN
   `(n + 1 - m = SUC (n - m)) /\ (n + 1 - (m + 1) = n - m)` by DECIDE_TAC THEN
   ASM_SIMP_TAC (srw_ss() ++ ARITH_ss) [GENLIST_CONS, GENLIST_FUN_EQ]);
 
-val listRange_EMPTY = store_thm(
-  "listRange_EMPTY",
+val listRangeINC_EMPTY = store_thm(
+  "listRangeINC_EMPTY",
   ``n < m ==> ([m .. n] = [])``,
-  SRW_TAC [][listRange_def] THEN
+  SRW_TAC [][listRangeINC_def] THEN
   `n + 1 - m = 0` by DECIDE_TAC THEN SRW_TAC[][]);
+
+val listRangeLHI_def = Define`
+  listRangeLHI m n = GENLIST (\i. m + i) (n - m)
+`;
+
+val _ = add_rule { block_style = (AroundEachPhrase, (PP.CONSISTENT, 0)),
+                   fixity = Closefix,
+                   paren_style = OnlyIfNecessary,
+                   pp_elements = [TOK "[", TM, HardSpace 1, TOK "..<",
+                                  BreakSpace(1,1), TM, BreakSpace(0,0),
+                                  TOK "]"],
+                   term_name = "listRangeLHI" }
+
+val listRangeLHI_EQ = store_thm(
+  "listRangeLHI_EQ",
+  ``[m ..< m] = []``,
+  SRW_TAC[][listRangeLHI_def]);
+
+val MEM_listRangeLHI = store_thm(
+  "MEM_listRangeLHI",
+  ``MEM x [m ..< n] <=> m <= x /\ x < n``,
+  SRW_TAC[ARITH_ss][listRangeLHI_def, MEM_GENLIST, EQ_IMP_THM] THEN
+  Q.EXISTS_TAC `x - m` THEN DECIDE_TAC);
+val _ = export_rewrites ["MEM_listRangeLHI"]
+
 
 val _ = export_theory();
